replacing string keys with int keys (#28)
* replacing string keys with int keys

* finish proof

bin/query/M.ml
@@ -1,5 +1,5 @@
 
-module SM = Map.Make(String)
+module SM = Map.Make(Uint63)
 
 type 'a t = 'a SM.t
 
@@ -8,13 +8,15 @@ let insert = SM.add
 let lookup = SM.find_opt
 let size = SM.cardinal
 let bindings = SM.bindings
-
+(* 
 let printMap m =
   SM.iter (fun key value -> Printf.printf "%s -> %d\n" key value) m
+ *)
 
-let tr_concat xss =
+(* let tr_concat xss =
   let rec aux acc ls =
     match ls with
     | [] -> acc
     | xs :: xss' -> aux (List.rev_append xs acc) xss'
   in aux [] xss
+ *)
