theory/Bear/RomanWheel.v
@@ -1,10 +1,12 @@
 Require Import List.
 Import ListNotations.
 
-Require Import String.
-Open Scope string_scope.
+Require Import PrimInt63.
+Require Import Uint63.
+Require Import ZArith.
+Require Import Lia.
 
-Require Import Games.Util.Show.
+Require Import Games.Util.IntHash.
 Require Import Games.Bear.Graph.
 Require Import Games.Bear.BearGame.
 Require Import Games.Game.TB.
@@ -39,40 +41,8 @@ Definition c_clockwise (s : Spoke) : Spoke :=
 Definition list_spokes :=
   [S1;S2;S3;S4;S5;S6;S7;S8].
 
-Definition str1 : string := "1".
-Definition str2 : string := "2".
-Definition str3 : string := "3".
-Definition str4 : string := "4".
-Definition str5 : string := "5".
-Definition str6 : string := "6".
-Definition str7 : string := "7".
-Definition str8 : string := "8".
-
-Definition show_spoke (s : Spoke) : string := (
-  match s with
-  | S1 => str1
-  | S2 => str2
-  | S3 => str3
-  | S4 => str4
-  | S5 => str5
-  | S6 => str6
-  | S7 => str7
-  | S8 => str8
-  end)%string.
-
 Inductive SpokeLoc :=
   Mid | L | R.
-
-Definition strM : string := "M".
-Definition strL : string := "L".
-Definition strR : string := "R".
-
-Definition show_loc (l : SpokeLoc) : string := (
-  match l with
-  | Mid => strM
-  | L => strL
-  | R => strR
-  end)%string.
 
 Definition list_locs :=
   [Mid;L;R].
@@ -81,118 +51,90 @@ Inductive RWVert :=
   | Center
   | SpokeVert (s : Spoke) (l : SpokeLoc).
 
-Lemma show_loc_inj : forall l l',
-  show_loc l = show_loc l' -> l = l'.
-Proof.
-  intros l l'.
-  destruct l, l'; simpl;
-  (discriminate || reflexivity).
-Qed.
-
-Lemma spoke_loc : forall s s' l l',
-  show_spoke s ++ show_loc l =
-  show_spoke s' ++ show_loc l' ->
-  s = s' /\ l = l'.
-Proof.
-  intros s s' l l' pf.
-  destruct s, s'; try inversion pf;
-  (split; [reflexivity|now apply show_loc_inj]).
-Qed.
-
-Definition strC : string := "C".
-Definition str1L : string := "1L".
-Definition str1M : string := "1M".
-Definition str1R : string := "1R".
-Definition str2L : string := "2L".
-Definition str2M : string := "2M".
-Definition str2R : string := "2R".
-Definition str3L : string := "3L".
-Definition str3M : string := "3M".
-Definition str3R : string := "3R".
-Definition str4L : string := "4L".
-Definition str4M : string := "4M".
-Definition str4R : string := "4R".
-Definition str5L : string := "5L".
-Definition str5M : string := "5M".
-Definition str5R : string := "5R".
-Definition str6L : string := "6L".
-Definition str6M : string := "6M".
-Definition str6R : string := "6R".
-Definition str7L : string := "7L".
-Definition str7M : string := "7M".
-Definition str7R : string := "7R".
-Definition str8L : string := "8L".
-Definition str8M : string := "8M".
-Definition str8R : string := "8R".
-
-Definition show_RWVert (v : RWVert) : string :=
+Definition hash_RWVert (v : RWVert) : int :=
   match v with
-  | Center => strC
-  | SpokeVert S1 L => str1L
-  | SpokeVert S1 Mid => str1M
-  | SpokeVert S1 R => str1R
-  | SpokeVert S2 L => str2L
-  | SpokeVert S2 Mid => str2M
-  | SpokeVert S2 R => str2R
-  | SpokeVert S3 L => str3L
-  | SpokeVert S3 Mid => str3M
-  | SpokeVert S3 R => str3R
-  | SpokeVert S4 L => str4L
-  | SpokeVert S4 Mid => str4M
-  | SpokeVert S4 R => str4R
-  | SpokeVert S5 L => str5L
-  | SpokeVert S5 Mid => str5M
-  | SpokeVert S5 R => str5R
-  | SpokeVert S6 L => str6L
-  | SpokeVert S6 Mid => str6M
-  | SpokeVert S6 R => str6R
-  | SpokeVert S7 L => str7L
-  | SpokeVert S7 Mid => str7M
-  | SpokeVert S7 R => str7R
-  | SpokeVert S8 L => str8L
-  | SpokeVert S8 Mid => str8M
-  | SpokeVert S8 R => str8R
+  | Center => 0
+  | SpokeVert S1 L => 1
+  | SpokeVert S1 Mid => 2
+  | SpokeVert S1 R => 3
+  | SpokeVert S2 L => 4
+  | SpokeVert S2 Mid => 5
+  | SpokeVert S2 R => 6
+  | SpokeVert S3 L => 7
+  | SpokeVert S3 Mid => 8
+  | SpokeVert S3 R => 9
+  | SpokeVert S4 L => 10
+  | SpokeVert S4 Mid => 11
+  | SpokeVert S4 R => 12
+  | SpokeVert S5 L => 13
+  | SpokeVert S5 Mid => 14
+  | SpokeVert S5 R => 15
+  | SpokeVert S6 L => 16
+  | SpokeVert S6 Mid => 17
+  | SpokeVert S6 R => 18
+  | SpokeVert S7 L => 19
+  | SpokeVert S7 Mid => 20
+  | SpokeVert S7 R => 21
+  | SpokeVert S8 L => 22
+  | SpokeVert S8 Mid => 23
+  | SpokeVert S8 R => 24
   end.
 
-Global Instance Show_RWVert : Show RWVert. refine {|
-  show := show_RWVert;
-  show_inj := _;
+Definition unhash_RWVert (z : Z) : option RWVert := (
+  match z with
+  | 0 => Some Center
+  | 1 => Some (SpokeVert S1 L)
+  | 2 => Some (SpokeVert S1 Mid)
+  | 3 => Some (SpokeVert S1 R)
+  | 4 => Some (SpokeVert S2 L)
+  | 5 => Some (SpokeVert S2 Mid)
+  | 6 => Some (SpokeVert S2 R)
+  | 7 => Some (SpokeVert S3 L)
+  | 8 => Some (SpokeVert S3 Mid)
+  | 9 => Some (SpokeVert S3 R)
+  | 10 => Some (SpokeVert S4 L)
+  | 11 => Some (SpokeVert S4 Mid)
+  | 12 => Some (SpokeVert S4 R)
+  | 13 => Some (SpokeVert S5 L)
+  | 14 => Some (SpokeVert S5 Mid)
+  | 15 => Some (SpokeVert S5 R)
+  | 16 => Some (SpokeVert S6 L)
+  | 17 => Some (SpokeVert S6 Mid)
+  | 18 => Some (SpokeVert S6 R)
+  | 19 => Some (SpokeVert S7 L)
+  | 20 => Some (SpokeVert S7 Mid)
+  | 21 => Some (SpokeVert S7 R)
+  | 22 => Some (SpokeVert S8 L)
+  | 23 => Some (SpokeVert S8 Mid)
+  | 24 => Some (SpokeVert S8 R)
+  | _ => None
+  end)%Z.
+
+Lemma unhash_hash : forall v,
+  unhash_RWVert (to_Z (hash_RWVert v)) = Some v.
+Proof.
+  destruct v as [|[] []]; reflexivity.
+Qed.
+
+Lemma hash_RWVert_inj : forall v v',
+  hash_RWVert v = hash_RWVert v' -> v = v'.
+Proof.
+  intros v v' pf1.
+  pose proof (unhash_hash v) as pf2.
+  rewrite pf1 in pf2.
+  rewrite unhash_hash in pf2.
+  congruence.
+Qed.
+
+Global Instance IntHash_RWVert : IntHash RWVert := {|
+  hash := hash_RWVert;
+  hash_inj := hash_RWVert_inj;
   |}.
-Proof.
-  - intros v v'.
-    destruct v as [|[] []];
-    destruct v' as [|[] []]; try reflexivity.
-    all: discriminate.
-Defined.
 
-Global Instance RWVert_Nonnil : Nonnil RWVert.
+Lemma hash_small : forall v,
+  (to_Z (hash v) < 2 ^ 5)%Z.
 Proof.
-  constructor.
-  destruct x; simpl.
-  - discriminate.
-  - destruct s; destruct l; discriminate.
-Qed.
-
-Global Instance RWVert_CommaFree : CommaFree RWVert.
-Proof.
-  constructor.
-  destruct x.
-  - simpl; repeat split; discriminate.
-  - unfold show.
-    unfold Show_RWVert.
-    destruct s, l; simpl;
-    repeat split; discriminate.
-Qed.
-
-Global Instance RWVert_Semicolon : SemicolonFree RWVert.
-Proof.
-  constructor.
-  destruct x.
-  - simpl; repeat split; discriminate.
-  - unfold show.
-    unfold Show_RWVert.
-    destruct s, l; simpl;
-    repeat split; discriminate.
+  intros [|[][ ]]; simpl; reflexivity.
 Qed.
 
 Lemma NoDup_list_locs : NoDup list_locs.
@@ -342,7 +284,419 @@ Proof.
         now inversion Heq.
 Defined.
 
-Global Instance Show_RWV : Show (Vert RomanWheel) :=
-  Show_RWVert.
+Global Instance IntHash_RWV : IntHash (Vert RomanWheel) :=
+  IntHash_RWVert.
+
+Definition add_vert (v : Vert RomanWheel) (i : int) : int :=
+  (hash v) lor (i << 5).
+
+Definition lsb (i : Z) (n : Z) : Z :=
+  i mod (2 ^ n).
+
+Fixpoint pow2 n : positive :=
+  match n with
+  | 0 => xH
+  | S m => xO (pow2 m)
+  end.
+
+Lemma pow2_correct : forall n,
+  2 ^ n = Pos.to_nat (pow2 n).
+Proof.
+  induction n.
+  - reflexivity.
+  - rewrite Nat.pow_succ_r'.
+    simpl pow2.
+    rewrite Pos2Nat.inj_xO.
+    lia.
+Qed.
+
+Lemma pow_pow2 : forall p,
+  (2 ^ p)%positive = pow2 (Pos.to_nat p).
+Proof.
+  intro p.
+  apply Pos2Nat.inj.
+  rewrite Pos2Nat.inj_pow.
+  apply pow2_correct.
+Qed.
+
+Lemma Pos_lor_add : forall n x y, (
+  x < pow2 n ->
+  Pos.lor x (pow2 n * y) = x + (pow2 n * y))%positive.
+Proof.
+  induction n.
+  - simpl; lia.
+  - simpl; intros x y x_small.
+    destruct x; simpl in *.
+    + f_equal.
+      apply IHn.
+      unfold Pos.lt in x_small.
+      unfold Pos.compare in x_small.
+      simpl in x_small.
+      rewrite Pos.compare_cont_Gt_Lt in x_small.
+      assumption.
+    + f_equal.
+      apply IHn.
+      assumption.
+    + f_equal.
+Qed.
+
+Lemma lor_add : forall n x y, (
+  0 <= n ->
+  0 <= x ->
+  0 <= y ->
+  x < 2 ^ n ->
+  Z.lor x (y * 2 ^ n) = x + (y * 2 ^ n))%Z.
+Proof.
+  intros.
+  rewrite Z.mul_comm.
+  destruct x.
+  - rewrite Z.lor_0_l.
+    lia.
+  - destruct y; try lia.
+    + rewrite Z.mul_0_r.
+      rewrite Z.lor_0_r; lia.
+    + destruct n; try lia.
+      rewrite <- Pos2Z.inj_pow in *.
+      rewrite <- Pos2Z.inj_mul.
+      simpl; f_equal.
+      rewrite pow_pow2 in *.
+      apply Pos_lor_add; assumption.
+  - lia.
+Qed.
+
+Lemma Pos_lor_small : forall n x y, (
+  x < pow2 n ->
+  y < pow2 n ->
+  Pos.lor x y < pow2 n)%positive.
+Proof.
+  induction n; intros; simpl in *.
+  - lia.
+  - unfold Pos.lt in *.
+    unfold Pos.compare in *.
+    destruct x, y; simpl in *.
+    + rewrite Pos.compare_cont_Gt_Lt in *.
+      apply IHn; assumption.
+    + rewrite Pos.compare_cont_Gt_Lt in *.
+      apply IHn; assumption.
+    + assumption.
+    + rewrite Pos.compare_cont_Gt_Lt in *.
+      apply IHn; assumption.
+    + apply IHn; assumption.
+    + now rewrite Pos.compare_cont_Gt_Lt.
+    + assumption.
+    + now rewrite Pos.compare_cont_Gt_Lt.
+    + reflexivity.
+Qed.
+
+Lemma lor_small : forall x y d, (
+  0 <= d ->
+  0 <= x ->
+  0 <= y ->
+  x < 2 ^ d ->
+  y < 2 ^ d ->
+  Z.lor x y < 2 ^ d)%Z.
+Proof.
+  intros x y d d_nn x_nn y_nn Hx Hy.
+  destruct x; try lia.
+  - now rewrite Z.lor_0_l.
+  - destruct y; try lia.
+    + now rewrite Z.lor_0_r.
+    + simpl.
+      destruct d; try lia.
+      rewrite <- Pos2Z.inj_pow in *.
+      apply Pos2Z.pos_lt_pos.
+      rewrite pow_pow2 in *.
+      apply Pos_lor_small; assumption.
+Qed.
+
+Definition get_vert (i : int) : option (Vert RomanWheel * int) :=
+  match unhash_RWVert (lsb (to_Z i) 5) with
+  | Some v => Some (v, i >> 5)%uint63
+  | None => None
+  end.
+
+Lemma get_vert_add_vert : forall v i d,
+  (to_Z i < 2^d)%Z ->
+  (0 <= d)%Z ->
+  (d + 5 <= 63)%Z ->
+  get_vert (add_vert v i) = Some (v, i).
+Proof.
+  intros.
+  unfold get_vert, add_vert.
+  rewrite lor_spec'.
+  rewrite lsl_spec.
+  unfold lsb.
+  rewrite (Z.mod_small _ wB).
+  - rewrite lor_add; try apply to_Z_bounded; try apply hash_small.
+    rewrite Z_mod_plus_full.
+    rewrite Z.mod_small.
+    + rewrite unhash_hash.
+      simpl Vert; do 2 f_equal.
+      apply to_Z_inj.
+      rewrite lsr_spec.
+      rewrite lor_spec'.
+      rewrite lsl_spec.
+      rewrite Z.mod_small.
+      * rewrite <- Z.shiftr_div_pow2; [|apply to_Z_bounded].
+        rewrite Z.shiftr_lor.
+        rewrite (Z.shiftr_div_pow2 (to_Z i * _)); [|apply to_Z_bounded].
+        rewrite Z.div_mul; [|vm_compute; lia].
+        rewrite Z.shiftr_eq_0; try apply to_Z_bounded.
+        -- apply Z.lor_0_l.
+        -- destruct (Z.eq_dec 0 (to_Z (hash v))).
+           ++ simpl Vert in *; rewrite <- e; reflexivity.
+           ++ rewrite <- Z.log2_lt_pow2.
+              ** apply hash_small.
+              ** destruct (to_Z_bounded (hash v)).
+                 simpl Vert in *; lia.
+      * split.
+        -- apply Z.mul_nonneg_nonneg; [|lia].
+           apply to_Z_bounded.
+        -- unfold wB.
+            simpl Z.of_nat.
+            apply (Z.lt_le_trans _ (2^(d+5))).
+            ++ rewrite Z.pow_add_r; simpl; lia.
+            ++ apply Z.pow_le_mono_r; lia.
+    + split.
+      * apply to_Z_bounded.
+      * apply hash_small.
+  - split.
+    + apply Z.mul_nonneg_nonneg; [|lia].
+      apply to_Z_bounded.
+    + unfold wB.
+      simpl Z.of_nat.
+      apply (Z.lt_le_trans _ (2^(d+5))).
+      * rewrite Z.pow_add_r; simpl; lia.
+      * apply Z.pow_le_mono_r; lia.
+Qed.
+
+Lemma add_vert_small v i d :
+  (0 <= d)%Z ->
+  (d + 5 <= 63)%Z ->
+  (to_Z i < 2^d)%Z ->
+  (to_Z (add_vert v i) < 2^(d+5))%Z.
+Proof.
+  intros d_nonneg d_small i_small.
+  unfold add_vert.
+  rewrite lor_spec'.
+  rewrite lsl_spec.
+  rewrite Z.mod_small.
+  - apply lor_small; try lia.
+    + apply to_Z_bounded.
+    + apply Z.mul_nonneg_nonneg; [|lia].
+      apply to_Z_bounded.
+    + apply (Z.lt_le_trans _ (2^5)).
+      * apply hash_small.
+      * apply Z.pow_le_mono_r; lia.
+    + rewrite Z.pow_add_r; try lia.
+      apply Zmult_gt_0_lt_compat_r; auto; lia.
+  - split.
+    + apply Z.mul_nonneg_nonneg; [|lia].
+      apply to_Z_bounded.
+    + apply (Z.lt_le_trans _ (2^(d+5))).
+      * rewrite Z.pow_add_r; try lia.
+        apply Zmult_gt_0_lt_compat_r; auto; lia.
+      * unfold wB, size.
+        apply Z.pow_le_mono_r; lia.
+Qed.
+
+Definition add_verts (vs : list (Vert RomanWheel)) (i : int) : int :=
+  fold_right add_vert i vs.
+
+Fixpoint get_verts n (i : int) : option (list (Vert RomanWheel)) :=
+  match n with
+  | 0 => Some []
+  | S m =>
+    match get_vert i with
+    | Some (v, j) =>
+      match get_verts m j with
+      | Some vs => Some (v :: vs)
+      | None => None
+      end
+    | None => None
+    end
+  end.
+
+Lemma add_verts_small vs i d :
+  (0 <= d)%Z ->
+  (d + 5 * Z.of_nat (length vs) <= 63)%Z ->
+  (to_Z i < 2^d)%Z ->
+  (to_Z (add_verts vs i) < 2^(d + 5 * Z.of_nat (length vs)))%Z.
+Proof.
+  intro d_nonneg.
+  unfold add_verts.
+  induction vs.
+  - simpl.
+    rewrite Z.add_0_r.
+    lia.
+  - simpl length.
+    rewrite Nat2Z.inj_succ.
+    rewrite <- Z.add_1_r.
+    simpl fold_right.
+    intro.
+    assert (d + 5 * (Z.of_nat (length vs) + 1) =
+      (d + 5 * (Z.of_nat (length vs))) + 5)%Z as pf by lia.
+    simpl Vert in pf.
+    rewrite pf.
+    intro Hi.
+    apply add_vert_small; simpl Vert; try lia.
+    apply IHvs; auto.
+    simpl Vert; lia.
+Qed.
+
+Lemma get_verts_add_verts : forall vs i d,
+  (to_Z i < 2^d)%Z ->
+  (0 <= d)%Z ->
+  (d + 5 * (Z.of_nat (length vs)) <= 63)%Z ->
+  get_verts (length vs) (add_verts vs i) = Some vs.
+Proof.
+  induction vs.
+  - intros; reflexivity.
+  - intros; simpl.
+    erewrite get_vert_add_vert.
+    + erewrite IHvs.
+      * reflexivity.
+      * exact H.
+      * auto.
+      * simpl length in H1.
+        simpl Vert. lia.
+    + apply add_verts_small; eauto.
+      simpl length in H1.
+      rewrite Nat2Z.inj_succ in H1.
+      rewrite <- Z.add_1_r in H1.
+      simpl Vert; lia.
+    + simpl length in H1.
+      rewrite Nat2Z.inj_succ in H1.
+      rewrite <- Z.add_1_r in H1.
+      simpl Vert; lia.
+    + simpl length in H1.
+      rewrite Nat2Z.inj_succ in H1.
+      rewrite <- Z.add_1_r in H1.
+      simpl Vert; lia.
+Qed.
+
+Definition add_player (p : Player.Player) (i : int) : int :=
+  match p with
+  | Player.White => i << 1
+  | Player.Black => 1 lor (i << 1)
+  end.
+
+Definition get_player (i : int) : Player.Player * int :=
+  match is_even i with
+  | true => (Player.White, i >> 1)
+  | false => (Player.Black, i >> 1)
+  end%uint63.
+
+Lemma lor_1_even : forall x : Z,
+  (0 <= x -> Z.even x = true -> Z.lor 1 x = x + 1)%Z.
+Proof.
+  intros x x_nonneg x_even.
+  unfold Z.lor.
+  destruct x; try lia.
+  rewrite Pos2Z.add_pos_pos.
+  destruct p; try discriminate.
+  reflexivity.
+Qed.
+
+Lemma get_player_add_player : forall p i,
+  (to_Z i < 2^62)%Z ->
+  get_player (add_player p i) = (p,i).
+Proof.
+  intros.
+  unfold get_player, add_player.
+  destruct p.
+  - rewrite is_even_lsl_1.
+    f_equal.
+    apply to_Z_inj.
+    rewrite lsr_spec.
+    rewrite lsl_spec.
+    rewrite Z.mod_small.
+    + simpl; unfold Z.pow_pos; simpl.
+      apply Z.div_mul; lia.
+    + split.
+      * apply Z.mul_nonneg_nonneg; [|lia].
+        apply to_Z_bounded.
+      * simpl; unfold Z.pow_pos; simpl.
+        unfold wB; simpl Z.of_nat.
+        lia.
+  - rewrite is_even_bit.
+    rewrite lor_spec; simpl.
+    f_equal.
+    apply to_Z_inj.
+    rewrite lsr_spec.
+    rewrite lor_spec'.
+    rewrite lsl_spec.
+    simpl Z.pow.
+    unfold Z.pow_pos; simpl Pos.iter.
+    rewrite Z.mod_small.
+    + rewrite lor_1_even.
+      * rewrite Z.div_add_l; [|lia].
+        unfold Z.div; simpl; lia.
+      * apply Z.mul_nonneg_nonneg; [|lia].
+        apply to_Z_bounded.
+      * rewrite Z.even_mul.
+        apply Bool.orb_true_r.
+    + split.
+      * apply Z.mul_nonneg_nonneg; [|lia].
+        apply to_Z_bounded.
+      * simpl; unfold Z.pow_pos; simpl.
+        unfold wB; simpl Z.of_nat.
+        lia.
+Qed.
+
+Definition hash_RW_State (s : BG_State RomanWheel) : int :=
+  match s with
+  | Build_BG_State _ p b hs _ _ _ _ =>
+      add_player p (add_vert b (add_verts hs 0))
+  end.
+
+Lemma hash_RW_State_inj : forall s s',
+  hash_RW_State s = hash_RW_State s' -> s = s'.
+Proof.
+  intros s s' Hss'.
+  unfold hash_RW_State in Hss'.
+  destruct s, s'; simpl in *.
+  pose proof (f_equal get_player Hss') as pf1.
+  rewrite get_player_add_player in pf1.
+  rewrite get_player_add_player in pf1.
+  - inversion pf1.
+    pose proof (f_equal get_vert H1) as pf2.
+    rewrite (get_vert_add_vert _ _ 15) in pf2; try lia.
+    rewrite (get_vert_add_vert _ _ 15) in pf2; try lia.
+    + inversion pf2.
+      pose proof (f_equal (get_verts (length hunters)) H3) as pf3.
+      rewrite (get_verts_add_verts _ 0 0) in pf3; try (lia||reflexivity).
+      rewrite hunters_3 in pf3.
+      rewrite <- hunters_0 in pf3.
+      rewrite (get_verts_add_verts _ 0 0) in pf3; try (lia||reflexivity).
+      * apply BG_State_ext; simpl; congruence.
+      * simpl Vert; rewrite hunters_0; lia.
+      * simpl Vert; rewrite hunters_3; lia.
+    + pose proof (add_verts_small hunters0 0 0).
+      simpl Vert in *.
+      rewrite hunters_0 in H.
+      apply H; simpl; [lia|lia |reflexivity].
+    + pose proof (add_verts_small hunters 0 0).
+      simpl Vert in *.
+      rewrite hunters_3 in H.
+      apply H; simpl; [lia|lia|reflexivity].
+  - apply (Z.lt_trans _ (2^20)); [|lia].
+    apply (add_vert_small _ _ 15); simpl; [lia|lia|].
+    pose (add_verts_small hunters0) as pf'.
+    simpl Vert in *.
+    rewrite hunters_0 in pf'.
+    apply (pf' _ 0)%Z; unfold to_Z; simpl; try lia.
+  - apply (Z.lt_trans _ (2^20)); [|lia].
+    apply (add_vert_small _ _ 15); simpl; [lia|lia|].
+    pose (add_verts_small hunters) as pf'.
+    simpl Vert in *.
+    rewrite hunters_3 in pf'.
+    apply (pf' _ 0)%Z; unfold to_Z; simpl; try lia.
+Qed.
+
+Global Instance IntHash_RW : IntHash (Game.GameState (BearGame RomanWheel)) := {|
+  hash := hash_RW_State;
+  hash_inj := hash_RW_State_inj;
+  |}.
 
 Definition RW_TB := Bear_TB RomanWheel.
