bin/gen/ExtractRomanWheel.v
@@ -6,6 +6,7 @@ Require Import Extraction.
 Require Import ExtrOcamlBasic.
 Require Import ExtrOcamlNatInt.
 Require Import ExtrOcamlNativeString.
+Require Import ExtrOCamlInt63.
 Extraction Language OCaml.
 
 Require Import Games.Util.OMap.
