theory/Util/IntHash.v
@@ -1,0 +1,25 @@
+Require Import Ascii.
+Open Scope char.
+
+Require Import PrimInt63.
+Require Import Uint63.
+Require Import Lia.
+Require List.
+Import List.ListNotations.
+
+Class IntHash (X : Type) : Type := {
+  hash : X -> int;
+  hash_inj : forall x x', hash x = hash x' -> x = x'
+  }.
+
+Definition IntHash_dec {X} `{IntHash X} : forall x x' : X,
+  {x = x'} + {x <> x'}.
+Proof.
+  intros.
+  destruct (eqb (hash x) (hash x')) eqn:Heq.
+  - rewrite eqb_spec in Heq.
+    left; now apply hash_inj.
+  - right; intro.
+    rewrite eqb_false_spec in Heq.
+    apply Heq; congruence.
+Defined.
